proofs/impls/array-map.bpl
@@ -83,21 +83,21 @@ function {:inline} postLP(called: [Invoc]bool, returned: [Invoc]bool, lin: SeqIn
 // ---------- Primitives for manipulating global state
 
 // Write to the table
-procedure {:atomic} {:layer 1} writeTable_spec(k, v: int)
+procedure {:atomic} {:layer 1} writeTable_atomic(k, v: int)
   modifies table;
 {
   table[k] := v;
 }
-procedure {:yields} {:layer 0} {:refines "writeTable_spec"}
+procedure {:yields} {:layer 0} {:refines "writeTable_atomic"}
   writeTable(k, v: int);
 
 // Read from the table
-procedure {:atomic} {:layer 1} readTable_spec(k: int)
+procedure {:atomic} {:layer 1} readTable_atomic(k: int)
   returns (v: int)
 {
   v := table[k];
 }
-procedure {:yields} {:layer 0} {:refines "readTable_spec"} readTable(k: int)
+procedure {:yields} {:layer 0} {:refines "readTable_atomic"} readTable(k: int)
   returns (v: int);
 
 
@@ -158,19 +158,15 @@ procedure {:yields} {:layer 1} {:refines "put_call_atomic"}
   ensures {:layer 1} preLP(called, returned, lin, this);
   modifies called;
 {
-  yield;
-  assert {:layer 1} tableInv(table, abs, tabvis, hb, lin, vis, tabLen, called, returned);
-  assert {:layer 1} (forall n1: Invoc :: hb[n1][this] ==> returned[n1]);
-  assert {:layer 1} (!called[this] && !returned[this]);
-
   call intro_writeCalled(this);
+
   yield;
   assert {:layer 1} tableInv(table, abs, tabvis, hb, lin, vis, tabLen, called, returned);
   assert {:layer 1} preLP(called, returned, lin, this);
 }
 
 
-procedure {:yields} {:layer 1} {:refines "put_spec"} put(k, v: int, {:linear "this"} this: Invoc)
+procedure {:yields} {:layer 1} {:refines "put_atomic"} put(k, v: int, {:linear "this"} this: Invoc)
   requires {:layer 1} tableInv(table, abs, tabvis, hb, lin, vis, tabLen, called, returned);
   requires {:layer 1} preLP(called, returned, lin, this);
   requires {:layer 1} invoc_m(this) == Map.put && invoc_k(this) == k && invoc_v(this) == v;
@@ -206,12 +202,6 @@ procedure {:yields} {:layer 1} {:refines "put_return_atomic"}
   ensures {:layer 1} tableInv(table, abs, tabvis, hb, lin, vis, tabLen, called, returned);
   modifies returned;
 {
-  yield;
-  assert {:layer 1} tableInv(table, abs, tabvis, hb, lin, vis, tabLen, called, returned);
-  assert {:layer 1} postLP(called, returned, lin, this);
-  assert {:layer 1} (forall n1: Invoc :: {vis[this][n1]}
-    vis[this][n1] ==> Set_ofSeq(lin)[n1]);
-
   call intro_writeReturned(this);
 
   yield;
@@ -230,18 +220,14 @@ procedure {:yields} {:layer 1} {:refines "get_call_atomic"}
   ensures {:layer 1} preLP(called, returned, lin, this);
   modifies called;
 {
-  yield;
-  assert {:layer 1} tableInv(table, abs, tabvis, hb, lin, vis, tabLen, called, returned);
-  assert {:layer 1} (forall n1: Invoc :: hb[n1][this] ==> returned[n1]);
-  assert {:layer 1} (!called[this] && !returned[this]);
-
   call intro_writeCalled(this);
+
   yield;
   assert {:layer 1} tableInv(table, abs, tabvis, hb, lin, vis, tabLen, called, returned);
   assert {:layer 1} preLP(called, returned, lin, this);
 }
 
-procedure {:yields} {:layer 1} {:refines "get_spec"} get(k: int, {:linear "this"} this: Invoc)
+procedure {:yields} {:layer 1} {:refines "get_atomic"} get(k: int, {:linear "this"} this: Invoc)
   returns (v: int)
   requires {:layer 1} tableInv(table, abs, tabvis, hb, lin, vis, tabLen, called, returned);
   requires {:layer 1} preLP(called, returned, lin, this);
@@ -260,6 +246,7 @@ procedure {:yields} {:layer 1} {:refines "get_spec"} get(k: int, {:linear "this"
   call my_vis := intro_readLin();
   call intro_writeVis(this, my_vis);
   call intro_writeLin(this);
+  call intro_writeRet(this, RetVal_ofInt(v));
 
   yield; assert {:layer 1} tableInv(table, abs, tabvis, hb, lin, vis, tabLen, called, returned)
     && postLP(called, returned, lin, this);
@@ -276,12 +263,6 @@ procedure {:yields} {:layer 1} {:refines "get_return_atomic"}
   ensures {:layer 1} tableInv(table, abs, tabvis, hb, lin, vis, tabLen, called, returned);
   modifies returned;
 {
-  yield;
-  assert {:layer 1} tableInv(table, abs, tabvis, hb, lin, vis, tabLen, called, returned);
-  assert {:layer 1} postLP(called, returned, lin, this);
-  assert {:layer 1} (forall n1: Invoc :: {vis[this][n1]}
-    vis[this][n1] ==> Set_ofSeq(lin)[n1]);
-
   call intro_writeReturned(this);
 
   yield;
@@ -300,18 +281,14 @@ procedure {:yields} {:layer 1} {:refines "contains_call_atomic"}
   ensures {:layer 1} preLP(called, returned, lin, this);
   modifies called;
 {
-  yield;
-  assert {:layer 1} tableInv(table, abs, tabvis, hb, lin, vis, tabLen, called, returned);
-  assert {:layer 1} (forall n1: Invoc :: hb[n1][this] ==> returned[n1]);
-  assert {:layer 1} (!called[this] && !returned[this]);
-
   call intro_writeCalled(this);
+
   yield;
   assert {:layer 1} tableInv(table, abs, tabvis, hb, lin, vis, tabLen, called, returned);
   assert {:layer 1} preLP(called, returned, lin, this);
 }
 
-procedure {:yields} {:layer 1} {:refines "contains_spec"}
+procedure {:yields} {:layer 1} {:refines "contains_atomic"}
     contains(v: int, {:linear "this"} this: Invoc)
   returns (res: bool, witness_k: int)
   requires {:layer 1} tableInv(table, abs, tabvis, hb, lin, vis, tabLen, called, returned);
@@ -369,6 +346,7 @@ procedure {:yields} {:layer 1} {:refines "contains_spec"}
 
       res := true;
 
+      call intro_writeRet(this, RetVal_ofBool(res));
       yield; assert {:layer 1} tableInv(table, abs, tabvis, hb, lin, vis, tabLen, called, returned)
         && postLP(called, returned, lin, this);
       assert {:layer 1} (forall n1: Invoc :: {vis[this][n1]}
@@ -401,6 +379,7 @@ procedure {:yields} {:layer 1} {:refines "contains_spec"}
 
   res := false;
 
+  call intro_writeRet(this, RetVal_ofBool(res));
   yield; assert {:layer 1} tableInv(table, abs, tabvis, hb, lin, vis, tabLen, called, returned)
     && postLP(called, returned, lin, this);
   assert {:layer 1} (forall n1: Invoc :: {vis[this][n1]}
@@ -416,12 +395,6 @@ procedure {:yields} {:layer 1} {:refines "contains_return_atomic"}
   ensures {:layer 1} tableInv(table, abs, tabvis, hb, lin, vis, tabLen, called, returned);
   modifies returned;
 {
-  yield;
-  assert {:layer 1} tableInv(table, abs, tabvis, hb, lin, vis, tabLen, called, returned);
-  assert {:layer 1} postLP(called, returned, lin, this);
-  assert {:layer 1} (forall n1: Invoc :: {vis[this][n1]}
-    vis[this][n1] ==> Set_ofSeq(lin)[n1]);
-
   call intro_writeReturned(this);
 
   yield;
